Fun, plus, if compatibility proved

src/Basics.v
@@ -38,5 +38,26 @@ Proof.
   * inversion H. destruct l.
     - exists [], a. reflexivity.
     - simpl in H1. epose (IHl (pred n) _). destruct e, H0. subst. rewrite H0.
-      exists (a::x), x0. apply app_comm_cons. Unshelve. simpl. lia. 
+      exists (a::x), x0. apply app_comm_cons. Unshelve. simpl. lia.
+Qed.
+
+Inductive list_biforall {T1 T2 : Type} (P : T1 -> T2 -> Prop) : list T1 -> list T2 -> Prop :=
+| biforall_nil : list_biforall P [] []
+| biforall_cons hd hd' tl tl' : P hd hd' -> list_biforall P tl tl' -> list_biforall P (hd::tl) (hd'::tl').
+
+Theorem indexed_to_biforall {T1 T2 : Type} : forall (P : T1 -> T2 -> Prop) (l1 : list T1) (l2 : list T2) (d1 : T1) (d2 : T2),
+   list_biforall P l1 l2 <-> (forall i, i < length l1 -> P (nth i l1 d1) (nth i l2 d2)) /\ length l1 = length l2.
+Proof.
+  split; intros.
+  * induction H.
+    - split; intros; auto. inversion H.
+    - destruct IHlist_biforall. split. 2: simpl; lia. destruct i; intros.
+      + exact H.
+      + apply H1. simpl in H3. lia.
+  * destruct H. revert H0 H. generalize dependent l2. generalize dependent d1.
+    generalize dependent d2. induction l1; intros.
+    - simpl in H0. apply eq_sym, length_zero_iff_nil in H0. subst. constructor.
+    - simpl in H0. apply element_exist in H0 as G. destruct G, H1. subst. inversion H0.
+      constructor. apply (H 0); simpl; lia. eapply IHl1; auto. intros. apply (H (S i)).
+      simpl. lia.
 Qed.
